{{%Localize command definitions

\chapter{Class 17}

$$ \llbracket \textup{skip} \rrbracket = \lambda \sigma . \sigma $$

$$ \llbracket \textup{assert } b \rrbracket = \lambda \sigma . \textup{ if } \llbracket b \rrbracket \sigma 
\textup{ then } \sigma \textup{ else fail} $$

$$ \llbracket c \rrbracket : \Sigma \rightarrow \Sigma_\bot $$

$$ \llbracket c \rrbracket : \Sigma \rightarrow \Sigma_\bot^\textup{fail} = \Sigma \cup \{ \textup{fail}, \bot \} $$

Operationally:

$$\inferrule
{ \langle b, \sigma \rangle \downarrow \top }
{ \langle \textup{assert } b, \sigma \rangle \downarrow \sigma }
$$

$$\inferrule
{ \langle b, \sigma \rangle \downarrow \bot }
{ \langle \textup{assert } b, \sigma \rangle \downarrow \textup{fail} }
$$

$$ \textup{wlp} ( \textup{skip}, \psi ) = \psi $$

$$ \textup{wlp} ( \textup{assert } b, \psi) = b \wedge \psi $$

$$ \{ b \wedge \psi \} \textup{ assert } b~ \{ \psi \} $$

$$ \llbracket c \rrbracket \subseteq \Sigma \times \Sigma_\bot^\textup{fail} $$

$$ \llbracket \textup{assume } b \rrbracket = \{ (\sigma, \sigma') \;|\; \sigma \vDash b \and \sigma' = \sigma \} $$

}} % End localization of command definitions
